proof/TypingRules.v
@@ -6,6 +6,7 @@ From PLF Require Import LinearContext.
 From PLF Require Import RfTypeDef.
 From PLF Require Import TypeClosedSimp.
 From PLF Require Import DenotationSimp.
+From PLF Require Import CtxErase.
 From PLF Require Import WellFormedSimp.
 From PLF Require Import TypeDisj.
 From PLF Require Import SubtypingSimp.
@@ -15,8 +16,11 @@ From Coq Require Import Lists.List.
 
 Import CoreLangSimp.
 Import LinearContext.
+Import NoDup.
+Import Nstate.
 Import TypeClosedSimp.
 Import DenotationSimp.
+Import CtxErase.
 Import WellFormedSimp.
 Import TypeDisj.
 Import SubtypingSimp.
@@ -33,20 +37,15 @@ Import ListNotations.
 (* Definition apply_op_from_cids (op: biop) (cid1 cid2: cid): tm := *)
 (* (apply_op op n1 n2). *)
 
-Definition const_order: constant -> constant -> Prop.
-Admitted.
-
-Lemma const_order_is_well_founded: well_founded const_order.
-Admitted.
-
 Reserved Notation "Gamma '\C-' t '\Tin' T" (at level 40).
 Reserved Notation "Gamma '\C-' t '\Vin' T" (at level 40).
 
 Inductive term_under_type_chek : context -> tm -> underty -> Prop :=
 | UT_Value: forall Gamma v uty, Gamma \C- v \Vin uty -> Gamma \C- (tvalue v) \Tin uty
 | UT_Exn: forall Gamma T, well_formed Gamma (mk_bot T) -> Gamma \C- texn \Tin (mk_bot T)
-| UT_Sub: forall Gamma e tau1 tau2,
+| UT_Sub: forall Gamma e (tau1 tau2:underty),
     well_formed Gamma tau2 ->
+    (* empty \N- e \Tin ou\_ tau1 _/ -> empty \N- e \Tin ou\_ tau2 _/ -> *)
     l_empty \C- e \Tin tau1 -> l_empty \C- tau1 \<: tau2 ->
     Gamma \C- e \Tin tau2
 | UT_Eq: forall Gamma e tau1 tau2,
@@ -65,8 +64,8 @@ Inductive term_under_type_chek : context -> tm -> underty -> Prop :=
 (* operators only take nat type *)
 | UT_LetOp: forall (Gamma: context) x op (v1 v2: cid) e tau, forall phi1 phi2,
     well_formed Gamma tau ->
-    Gamma \C- v1 \Vin ([[v: TNat | phi1 ]]) ->
-    Gamma \C- v2 \Vin ([[v: TNat | phi2 ]]) ->
+    Gamma \C- v1 \Vin ([[v: fst_ty_of_op op | phi1 ]]) ->
+    Gamma \C- v2 \Vin ([[v: snd_ty_of_op op | phi2 ]]) ->
     (Gamma <l> x :l: (mk_op_retty_from_cids op v1 v2)) \C- e \Tin tau ->
     Gamma \C- (tletbiop x op v1 v2 e) \Tin tau
 | UT_LetAppIndepend: forall Gamma x v1 v2 e tau, forall tauarg tau_x,
@@ -82,11 +81,13 @@ Inductive term_under_type_chek : context -> tm -> underty -> Prop :=
     Gamma \C- (tletapp x v1 c2 e) \Tin tau
 | UT_Matchb_true: forall Gamma v e1 e2 tau,
     well_formed Gamma tau ->
-    Gamma \C- v \Vin (mk_eq_constant true) -> Gamma \C- e1 \Tin tau ->
+    Gamma \C- v \Vin (mk_eq_constant true) ->
+    Gamma \C- e1 \Tin tau -> (erase_ctx Gamma) \N- e2 \Tin ou\_ tau _/ ->
     Gamma \C- (tmatchb v e1 e2) \Tin tau
 | UT_Matchb_false: forall Gamma v e1 e2 tau,
     well_formed Gamma tau ->
-    Gamma \C- v \Vin (mk_eq_constant false) -> Gamma \C- e2 \Tin tau ->
+    Gamma \C- v \Vin (mk_eq_constant false) ->
+    Gamma \C- e2 \Tin tau -> (erase_ctx Gamma) \N- e1 \Tin ou\_ tau _/ ->
     Gamma \C- (tmatchb v e1 e2) \Tin tau
 with value_under_type_check : context -> value -> underty -> Prop :=
 | UT_Contant: forall Gamma (c: constant),
@@ -112,11 +113,18 @@ with value_under_type_check : context -> value -> underty -> Prop :=
     well_formed Gamma ((t1 u--> t2) u--> tau) ->
     (Gamma <l> x :l: Uty (t1 u--> t2)) \C- e \Tin tau ->
     Gamma \C- (vlam x (u\_ (t1 u--> t2) _/) e) \Vin ((t1 u--> t2) u--> tau)
+| UT_LamFix: forall Gamma x T phi f e tau,
+    well_formed Gamma (x o: {{v:T | phi}} o--> tau) ->
+    Gamma \C- (vlam x T (vlam f (T t--> u\_ tau _/) e)) \Vin (x o: {{v:T | phi}} o--> ((x o: {{v:T | well_founded_constraint x phi}} o--> tau) u--> tau)) ->
+    Gamma \C- (vfix f (T t--> u\_ tau _/) x T e) \Vin (x o: {{v:T | phi}} o--> tau)
 where
 "Gamma '\C-' t '\Tin' T" := (term_under_type_chek Gamma t T) and "Gamma '\C-' t '\Vin' T" := (value_under_type_check Gamma t T).
 
 Scheme value_under_type_check_rec := Induction for value_under_type_check Sort Prop
     with term_under_type_chek_rec := Induction for term_under_type_chek Sort Prop.
+
+Global Hint Constructors term_under_type_chek: core.
+Global Hint Constructors value_under_type_check: core.
 
 (* Definition mk_op_retty_spec: forall Gamma op (cid1 cid2: cid) (phi1 phi2: refinement), *)
 (*     ctx_inv Gamma -> *)
@@ -135,6 +143,87 @@ Qed.
 
 Global Hint Resolve type_judgement_implies_inv: core.
 
+Lemma type_judgement_implies_no_dup: forall Gamma e tau,
+    Gamma \C- e \Tin tau -> type_ctx_no_dup empty Gamma.
+Proof.
+  intros. apply type_judgement_implies_inv in H... destruct H... apply ctx_inv_implies_no_dup in H...
+  rewrite nstate_to_tystate_empty in H... apply H.
+Qed.
+
+Global Hint Resolve type_judgement_implies_no_dup: core.
+
+(* Lemma lam_has_type_tm_to_value: forall Gamma y T' e tau0, *)
+(*     Gamma \C- vlam y T' e \Tin tau0 -> Gamma \C- vlam y T' e \Vin tau0. *)
+(* Proof with eauto. *)
+(*   intros. *)
+(*   assert (well_formed_type tau0). apply type_judgement_implies_inv in H... destruct H... *)
+(*   induction tau0; try inversion H4; subst. *)
+(*   - admit. *)
+(*   - admit. *)
+(*   - inversion H. *)
+(*     inversion H; subst. *)
+(*     + inversion H3... *)
+(*     + inversion H3; subst. inversion H8... *)
+(*     + *)
+(*     + apply subtyping_same_ty in H3. simpl in H3. subst. *)
+
+(*   inversion H; subst... *)
+(*   - destruct H0. assert (well_formed_type tau0)... *)
+(*     induction tau0; try inversion H4; subst. *)
+(*     + inversion H1; subst. *)
+(*     induction H4... *)
+
+(*     destruct H3. *)
+
+(*     eapply is_subtype_spec... in H2... *)
+Lemma type_judgement_implies_lam_var_not_in_Gamma: forall Gamma x T e tau,
+    Gamma \C- vlam x T e \Vin tau -> l_find_right_most Gamma x = None.
+Proof with eauto.
+  intros...
+  inversion H; subst.
+  + apply type_judgement_implies_inv in H6. destruct H6...
+  + apply type_judgement_implies_inv in H6. destruct H6...
+Qed.
+
+(* Function Renaming Axiom *)
+Lemma Function_Renaming_Axiom: forall Gamma x T e tau,
+    Gamma \C- vlam x T e \Tin tau -> l_find_right_most Gamma x = None.
+Admitted.
+
+(* Renaming Axiom *)
+Lemma Function_Renaming_Axiom2: forall Gamma x T y T' e tau,
+    Gamma \C- vlam x T (vlam y T' e) \Vin tau ->
+    l_find_right_most Gamma x = None /\ l_find_right_most Gamma y = None /\ y <> x.
+Admitted.
+(* Proof with eauto. *)
+(*   intros... *)
+(*   inversion H; subst. *)
+(*   + apply Function_Renaming_Axiom in H. split... *)
+(*     inversion H2; subst... *)
+(*     assert (Gamma \C- vlam x T (vlam y T' e) \Tin tau)... apply Function_Renaming_Axiom in H0... split... *)
+(*   + apply type_judgement_implies_lam_var_not_in_Gamma in H. split... apply lam_has_type_tm_to_value in H6. *)
+(*     apply type_judgement_implies_lam_var_not_in_Gamma in H6. split... *)
+(* Qed. *)
+
 Lemma type_judgement_implies_basic_type_judgement: forall Gamma e tau,
     Gamma \C- e \Tin tau -> (erase_ctx Gamma) \N- e \Tin u\_ tau _/.
-Admitted.
+Proof with eauto.
+  apply (term_under_type_chek_rec (fun Gamma v tau HvT => (erase_ctx Gamma) \N- v \Vin u\_ tau _/));
+    (try eapply mk_op_has_type; eauto); intros...
+  - simpl...
+  - destruct e... apply over_eq_var_in_Gamma_has_type in H...
+  - destruct e... apply under_eq_var_in_Gamma_has_type in H...
+  - apply var_in_Gamma_has_type in e...
+  - eapply var_in_Gamma_has_type in e...
+  - erewrite no_dup_implies_ctx_lift in H... destruct tau_x... simpl...
+  - destruct w. constructor... erewrite no_dup_implies_ctx_lift in H...
+  - destruct w. constructor... simpl in H. inversion H; subst. inversion H4; subst. inversion H5; subst.
+    rewrite update_permute... apply Function_Renaming_Axiom2 in v... destruct v... destruct H3...
+  - apply subtyping_same_ty in i. simpl in i. rewrite <- i. eapply weakening...
+  - apply subtyping_same_ty in i. simpl in i. rewrite <- i...
+  - apply disj_same_ty in d... destruct d. rewrite <- H1...
+  - erewrite no_dup_implies_ctx_lift in H0...
+  - erewrite no_dup_implies_ctx_lift in H1...
+  - erewrite no_dup_implies_ctx_lift in H1...
+  - erewrite no_dup_implies_ctx_lift in H1... simpl in H1... rewrite under_subst_cid_preserve_ty in H1...
+Qed.
