proof/CtxErase.v
@@ -1,0 +1,69 @@
+(** * MoreStlc: More on the Simply Typed Lambda-Calculus *)
+
+Set Warnings "-notation-overridden,-parsing".
+From PLF Require Import Maps.
+From PLF Require Import CoreLangSimp.
+From PLF Require Import NormalTypeSystemSimp.
+From PLF Require Import LinearContext.
+From PLF Require Import RfTypeDef.
+From PLF Require Import TypeClosedSimp.
+From PLF Require Import TermOrdering.
+From PLF Require Import DenotationSimp.
+From Coq Require Import Logic.FunctionalExtensionality.
+From Coq Require Import Logic.ClassicalFacts.
+From Coq Require Import Lists.List.
+From Coq Require Import FunInd.
+From Coq Require Import Recdef.
+
+Import CoreLangSimp.
+Import NormalTypeSystemSimp.
+Import LinearContext.
+Import RfTypeDef.
+Import TypeClosedSimp.
+Import Nstate.
+Import NoDup.
+Import DenotationSimp.
+Import ListNotations.
+
+(* Work only when there is no dup in Gamma! *)
+Fixpoint erase_ctx (Gamma: lcontxt) :=
+  match Gamma with
+  | nil => empty
+  | (x, tau)::Gamma => update (erase_ctx Gamma) x (ou\_ tau _/)
+  end.
+
+Lemma erase_included: forall Gamma, includedin empty (erase_ctx Gamma).
+Admitted.
+
+Global Hint Resolve erase_included: core.
+
+Lemma no_dup_implies_ctx_lift: forall Gamma x tau_x e tau,
+    type_ctx_no_dup empty (Gamma <l> x :l: tau_x) ->
+    (erase_ctx (Gamma <l> x :l: tau_x)) \N- e \Tin tau <-> (erase_ctx ((x, tau_x) :: Gamma)) \N- e \Tin tau.
+Admitted.
+
+Global Hint Resolve no_dup_implies_ctx_lift: core.
+
+Lemma over_eq_var_in_Gamma_has_type: forall Gamma x T phi,
+    l_find_right_most Gamma x = Some (Oty ({{v: T | phi }})) -> (erase_ctx Gamma) \N- x \Vin T.
+Admitted.
+
+Global Hint Resolve over_eq_var_in_Gamma_has_type: core.
+
+Lemma under_eq_var_in_Gamma_has_type: forall Gamma x T phi,
+    l_find_right_most Gamma x = Some (Uty ([[v: T | phi ]])) -> (erase_ctx Gamma) \N- x \Vin T.
+Admitted.
+
+Global Hint Resolve under_eq_var_in_Gamma_has_type: core.
+
+Lemma var_in_Gamma_has_type: forall Gamma x tau,
+    l_find_right_most Gamma x = Some tau -> (erase_ctx Gamma) \N- x \Vin (ou\_ tau _/).
+Admitted.
+
+Global Hint Resolve var_in_Gamma_has_type: core.
+
+Lemma tmR_in_ctx_aux_implies_has_type: forall Gamma st tau e,
+    tmR_in_ctx_aux st Gamma tau e -> (erase_ctx Gamma) \N- e \Tin ou\_ tau _/.
+Admitted.
+
+Global Hint Resolve tmR_in_ctx_aux_implies_has_type: core.
